{
 "cells": [
  {
   "cell_type": "markdown",
   "metadata": {},
   "source": [
    "# DSCI6001-5.4 Lecture\n",
    "\n",
    "### Assigned Reading: Kreyszig 9.6 ( use supplemental material)\n",
    "\n",
    "### Advanced Reading: Kreyszig 9.7, 9.8, 9.9\n",
    "\n",
    "## By the End of this Lecture You Will:\n",
    "\n",
    "1. Know what a composite function is\n",
    "2. Know how to use the Chain Rule for a total derivative\n",
    "3. Know what a partial derivative is and how to apply it\n",
    "4. Be able to use the Chain Rule for Partial Derivatives\n"
   ]
  },
  {
   "cell_type": "markdown",
   "metadata": {},
   "source": [
    "## Composite Functions\n",
    "\n",
    "The theory of functions is a really deep rabbithole and we cannot spend too much time on them. Many functions can be *de-composed* or **decomposed** as a composite, or grouping, of several other more *elementary* [functions]. This is a very helpful way to think of calculus in general. \n",
    "\n",
    "We say a given function $h(x)$ is equal to $f(x)$ composed of $g(x)$:\n",
    "\n",
    "$$h(x) = f \\circ g = f(g(x))$$\n",
    "\n",
    "This is to say simply that the inputs of $f(x)$ are the outputs of $g(x)$. Obviously with non-bijective functions, a number of functions with relatively crazy domains and ranges are possible. \n",
    "\n",
    "### Example:\n",
    "\n",
    "$g(x) = 4x^2$\n",
    "\n",
    "$f(x) = e^x$\n",
    "\n",
    "$f \\circ g = e^{4x^2}$\n",
    "\n",
    "### QUIZ:\n",
    "\n",
    "With the above problem is $f \\circ g = g \\circ f$? Can you think of some functions where this *is* true?\n",
    "\n"
   ]
  },
  {
   "cell_type": "markdown",
   "metadata": {},
   "source": [
    "## Chain Rule\n",
    "\n",
    "Derivatives can help us get around the issue of domains and ranges a bit.\n",
    "Suppose $f(x) = \\sqrt{x^2 + 1}$ and $g(x) = 2x + 1$, and we have\n",
    "\n",
    "$$y = f(g(x)) = \\sqrt{(2x+1)^2 + 1}$$\n",
    "\n",
    "If $f$ and $g$ are differentiable, then so is the composite function. The derivative of the composit function can be obtained using _chain rule_:\n",
    "\n",
    "If $y=f(u)$ is a differentiable function of $u$ and $u=g(x)$ is in turn a differentiable function of  $x$, then the composit function $y=f(g(x))$ is a differentiable function of $x$ whose derivative is given by the product\n",
    "\n",
    "$$\\frac{dy}{dx} = \\frac{dy}{du}\\frac{du}{dx}$$\n",
    "\n",
    "\n",
    "or, equivalently, by\n",
    "\n",
    "$$\\frac{dy}{dx} = f'(g(x)) g'(x)$$\n",
    "\n",
    "\n",
    "#### Example\n",
    "\n",
    "We want to find the derivative of the function:\n",
    "\n",
    "$$y=f(x) = (x^2+2)^2 - 3 (x^2+2) + 1$$\n",
    "\n",
    "Note that $y = u^2 - 3 u + 1$, where $u = x^2 + 2$. Thus\n",
    "\n",
    "$$ \\frac{dy}{du} = 2 u - 3 ~~~~~~~~~ \\text{and}~~~~~~~~~~ \\frac{du}{dx} = 2x$$\n",
    "\n",
    "and according to the chain rule:\n",
    "\n",
    "$$\\frac{dy}{dx} = \\frac{dy}{du}\\frac{du}{dx} = (2u-3)(2x) = [2(x^2+2) - 3](2x) = 2x(2x^2+1)$$\n",
    "\n",
    "#### Conceptual Insight\n",
    "\n",
    "The key aspect of the chain rule is that *rates of change multiply.* To illustrate, suppose that your salary increases twice as fast as your friend's. If your friend's salary increases \\$4000 per year, your salary will increase at the rate of 2$\\times$4000 or \\$8000 per year. In terms of derivatives,\n",
    "\n",
    "$$\\frac{d(\\text{your salary})}{dt} = \\frac{d(\\text{your salary})}{d(\\text{friend's salary})} \\times \\frac{d(\\text{friend's salary})}{dt}$$\n",
    "\n",
    "$$ $8000/\\text{yr} = 2 \\times $4000/\\text{yr}$$\n",
    "\n",
    "As another example, imagine a circle whose radius increases at a rate of $3~cm/s$. We can find the rate at which the area is increasing using the chain rule:\n",
    "\n",
    "$$\\frac{dA}{dt} = \\frac{dA}{dr} \\frac{dr}{dt}$$\n",
    "\n",
    "We're given the rate $dr/dt$, namely $dr/dt = 3~cm/s$. To compute $dA/dr$, we use the formula for the area of the circle, $A = \\pi r^2$.\n",
    "\n",
    "$$\\frac{dA}{dr} = \\frac{d}{dr}(\\pi r^2) = 2\\pi r$$\n",
    "\n",
    "\n",
    "Because, $dr/dt = 3~cm/s$, we obtain\n",
    "\n",
    "$$\\frac{dA}{dt} = (2\\pi r)(3) = 6\\pi r ~ cm^2/s$$\n",
    "\n",
    "\n",
    "### QUIZ:\n",
    "\n",
    "The cost of producing $x$ units of a particular commodity is $C(x) = \\frac{1}{3}x^2 + 4x + 53$ dollars, and the production level $t$ hours into a particular produciton run is $x(t) = 0.2 t^2 + 0.03 t$ units. At what rate is cost changing with respect to time after 4 hours?\n",
    "\n",
    "We find that\n",
    "\n",
    "$$\\frac{dC}{dx} = \\dfrac{2}{3}x + 4$$\n",
    "\n",
    "and \n",
    "\n",
    "$$\\frac{dx}{dt} = 0.4 t + 0.03$$\n",
    "\n",
    "so according to the chain rule\n",
    "\n",
    "$$\\frac{dC}{dt} = \\frac{dC}{dx} \\frac{dx}{dt} = \\left( \\frac{2}{3}x + 4\\right) (0.4 t + 0.03)$$\n",
    "\n",
    "When $t=4$, the level of production is\n",
    "\n",
    "$$x(4) = 0.2(4)^2 + 0.03(4) = 3.32~\\text{units}$$\n",
    "\n",
    "and by substituting $t=4$ and $x=3.32$ into the formula for $dC/dt$, we get\n",
    "\n",
    "$$\\left. \\frac{dC}{dt}\\right|_{t=4} = \\left[ \\frac{2}{3} (3.32) + 4 \\right][0.4(4) + 0.03] = 10.77$$"
   ]
  },
  {
   "cell_type": "markdown",
   "metadata": {},
   "source": [
    "## Chain Rule for Composite Functions\n",
    "\n",
    "If $z=f(x,y)$ is a function of variables $x$ and $y$ with partial derivativs $f_x$ and $f_y$, and if $x$ and $y$ are differentiable functions of another varialbe $t$, i.e., $x=g(t)$ and $y=h(t)$, then $z$ is also a function of $t$. In this case, we can find the _total derivative_ of $z$ w.r.t to $t$ given by\n",
    "\n",
    "$$\\frac{dz}{dt} = \\frac{\\partial z}{\\partial x} \\frac{dx}{dt} + \\frac{\\partial z}{\\partial y} \\frac{dy}{dt}$$\n",
    "\n",
    "Note that the expression for $dz/dt$ is the sum of two terms, each of which can ï¿¼be interpreted using the chain rule for a function of one variable.\n",
    "\n",
    "$$\\frac{\\partial z}{\\partial x} \\frac{dx}{dt} = \\text{rate of change of $z$ with respect to $t$ for fixed $y$}$$\n",
    "\n",
    "$$\\frac{\\partial z}{\\partial y} \\frac{dy}{dt} = \\text{rate of change of $z$ with respect to $t$ for fixed $x$}$$\n",
    "\n",
    "The chain rule for partial derivatives says that the total rate of change of $z$ with respect to $t$ is the sum of these two _partial_ rates of change.\n",
    "\n",
    "The above definition can be extended to functions of more than two variables. If $w=f(x,y,z,...)$ is a function of several varialbes, $x,y,z,...$, which in turn are functions of variable $t$, then the total derivative of $w$ is\n",
    "\n",
    "$$\\frac{dw}{dt} = \\frac{\\partial w}{\\partial x} \\frac{dx}{dt} + \\frac{\\partial w}{\\partial y} \\frac{dy}{dt} + \\frac{\\partial w}{\\partial z} \\frac{dz}{dt} + \\cdots$$\n",
    "\n",
    "\n",
    "#### Example 1\n",
    "\n",
    "Find $dz/dt$, given $z=x^2 + 3 x y + 2 y^2$; $x = t^2$, $y = 2t+1$.\n",
    "\n",
    "Solution:\n",
    "\n",
    "$$\\frac{\\partial z}{\\partial x} = 2 x + 3,~~~~ \\frac{\\partial z}{\\partial y} = 3x + 4 y$$\n",
    "\n",
    "$$\\frac{dx}{dt} = 2 t, ~~~~ \\frac{dy}{dt} = 2$$\n",
    "\n",
    "\n",
    "Using\n",
    "$$\\frac{dz}{dt} = \\frac{\\partial z}{\\partial x} \\frac{dx}{dt} + \\frac{\\partial z}{\\partial y} \\frac{dy}{dt}$$\n",
    "\n",
    "We get,\n",
    "$$\\frac{dz}{dt} = (2 x + 3)(2t) + (3x + 4y)(2) = (2 t^2 + 3)(2t) + (3 t^2 + 4(2t+1))(2)$$\n",
    "\n",
    "$$\\frac{dz}{dt} = 2(2 t^3 + 3 t^2 + 7 t + 4)$$\n",
    "\n",
    "Note that the total derivative is a function of $t$.\n",
    "\n",
    "\n",
    "#### Example 2\n",
    "\n",
    "Find (a) $\\frac{dz}{dx}$ and (b) $\\frac{dz}{dy}$, given $z=f(x,y) = x y^2 + x^2 y$, $y = \\ln x$.\n",
    "\n",
    "(a) Here $x$ is the independent variable. So we'll modify the chain rule as:\n",
    "\n",
    "$$\\frac{dz}{dx} = \\frac{\\partial z}{\\partial x} + \\frac{\\partial z}{\\partial y}\\frac{dy}{dx}$$\n",
    "\n",
    "$$\\frac{\\partial z}{\\partial x} = y^2 + 2 x y, \\frac{\\partial z}{\\partial y} = 2 x y + x^2, \\frac{dy}{dx} = \\frac{1}{x}$$\n",
    "\n",
    "Putting it all together, we get:\n",
    "\n",
    "$$\\frac{d z}{d x} = (y^2 + 2 x y) + (2 x y + x^2)\\frac{1}{x} = y^2 + 2xy + 2y +x$$\n",
    "\n",
    "(b) Here $y$ is the independent variable:\n",
    "\n",
    "$$\\frac{dz}{dy} = \\frac{\\partial z}{\\partial x}\\frac{dx}{dy} + \\frac{\\partial z}{\\partial y}$$\n",
    "\n",
    "Since $y = \\ln x$, this implise $x = e^y$. Therefore,\n",
    "\n",
    "$$\\frac{dx}{dy} = \\frac{d}{dy}(e^y) = e^y = x$$\n",
    "\n",
    "Thus\n",
    "\n",
    "$$\\frac{dz}{dy} = (y^2 + 2 x y) x + (2 x y + x^2) = x y^2 + 2 x^2 y + 2 x y + x^2$$"
   ]
  },
  {
   "cell_type": "markdown",
   "metadata": {},
   "source": [
    "## Assigned Problems:\n",
    "Kreyszig 9.6: All problems (Do 10 with a friend)"
   ]
  },
  {
   "cell_type": "code",
   "execution_count": null,
   "metadata": {
    "collapsed": true
   },
   "outputs": [],
   "source": []
  }
 ],
 "metadata": {
  "kernelspec": {
   "display_name": "Python 3",
   "language": "python",
   "name": "python3"
  },
  "language_info": {
   "codemirror_mode": {
    "name": "ipython",
    "version": 3
   },
   "file_extension": ".py",
   "mimetype": "text/x-python",
   "name": "python",
   "nbconvert_exporter": "python",
   "pygments_lexer": "ipython3",
   "version": "3.3.5"
  }
 },
 "nbformat": 4,
 "nbformat_minor": 0
}
